Update escrow bytecode (solc optimized) and add calldatasize to insts

example/Escrow.thy
@@ -1,10 +1,7 @@
 theory Escrow
 
 imports
-  "../Parse"
-  "../Hoare/HoareTripleForBasicBlocks"
-  "./ToyExamplesBlocks"
-  "../Word_Lib/Word_Lemmas_32"
+  Dispatcher
 begin
 (*
 pragma solidity ^0.4.0;
@@ -36,7 +33,7 @@ contract EscrowWallet {
 }
 
 Compiled with:
- solc --overwrite -o escrow-data --bin-runtime --asm --hashes escrow.sol
+ solc --optimize --overwrite -o escrow --bin-runtime --asm --hashes escrow.sol
 
 8f9595d4: addfund()
 1b9265b8: pay()
@@ -44,95 +41,134 @@ Compiled with:
 
 
 *)
-value"(parse_bytecode ''60606040526000357c0100000000000000000000000000000000000000000000000000000000900463ffffffff1680631b9265b814610053578063590e1ae3146100685780638f9595d41461007d57600080fd5b341561005e57600080fd5b610066610087565b005b341561007357600080fd5b61007b61011e565b005b6100856101b4565b005b600260009054906101000a900473ffffffffffffffffffffffffffffffffffffffff1673ffffffffffffffffffffffffffffffffffffffff163373ffffffffffffffffffffffffffffffffffffffff161415156100e357600080fd5b600160009054906101000a900473ffffffffffffffffffffffffffffffffffffffff1673ffffffffffffffffffffffffffffffffffffffff16ff5b600260009054906101000a900473ffffffffffffffffffffffffffffffffffffffff1673ffffffffffffffffffffffffffffffffffffffff163373ffffffffffffffffffffffffffffffffffffffff1614151561017a57600080fd5b6000809054906101000a900473ffffffffffffffffffffffffffffffffffffffff1673ffffffffffffffffffffffffffffffffffffffff16ff5b6000809054906101000a900473ffffffffffffffffffffffffffffffffffffffff1673ffffffffffffffffffffffffffffffffffffffff163373ffffffffffffffffffffffffffffffffffffffff1614151561020f57600080fd5b5600a165627a7a72305820cd7938db5bada113de91ec979b4dca8fdcb3c616a00562a67f5c288a71c479d10029'')"
+value"(parse_bytecode ''6060604052600436106100565763ffffffff7c01000000000000000000000000000000000000000000000000000000006000350416631b9265b8811461005b578063590e1ae3146100705780638f9595d414610083575b600080fd5b341561006657600080fd5b61006e61008b565b005b341561007b57600080fd5b61006e6100ce565b61006e610111565b6002543373ffffffffffffffffffffffffffffffffffffffff9081169116146100b357600080fd5b60015473ffffffffffffffffffffffffffffffffffffffff16ff5b6002543373ffffffffffffffffffffffffffffffffffffffff9081169116146100f657600080fd5b60005473ffffffffffffffffffffffffffffffffffffffff16ff5b6000543373ffffffffffffffffffffffffffffffffffffffff90811691161461013957600080fd5b5600a165627a7a723058207bd2ee8051b098c799df41466599cd311e376fd36372f2becec08fe494ba3cc10029'')"
 
 definition insts_ex where
-"insts_ex == [Stack (PUSH_N [0x60]), Stack (PUSH_N [0x40]), Memory MSTORE, Stack (PUSH_N [0]), Stack CALLDATALOAD,
+"insts_ex == [Stack (PUSH_N [0x60]), Stack (PUSH_N [0x40]), Memory MSTORE, Stack (PUSH_N [4]), Info CALLDATASIZE,
+  Arith inst_LT, Stack (PUSH_N [0, 0x56]), Pc JUMPI, Stack (PUSH_N [0xFF, 0xFF, 0xFF, 0xFF]),
   Stack (PUSH_N [1, 0, 0, 0, 0, 0, 0, 0, 0, 0, 0, 0, 0, 0, 0, 0, 0, 0, 0, 0, 0, 0, 0, 0, 0, 0, 0, 0, 0]),
-  Swap 0, Arith DIV, Stack (PUSH_N [0xFF, 0xFF, 0xFF, 0xFF]), Bits inst_AND, Dup 0,
-  Stack (PUSH_N [0x1B, 0x92, 0x65, 0xB8]), Arith inst_EQ, Stack (PUSH_N [0, 0x53]), Pc JUMPI, Dup 0,
-  Stack (PUSH_N [0x59, 0xE, 0x1A, 0xE3]), Arith inst_EQ, Stack (PUSH_N [0, 0x68]), Pc JUMPI, Dup 0,
-  Stack (PUSH_N [0x8F, 0x95, 0x95, 0xD4]), Arith inst_EQ, Stack (PUSH_N [0, 0x7D]), Pc JUMPI,
-  Stack (PUSH_N [0]), Dup 0, Unknown 0xFD, Pc JUMPDEST, Info CALLVALUE, Arith ISZERO,
-  Stack (PUSH_N [0, 0x5E]), Pc JUMPI, Stack (PUSH_N [0]), Dup 0, Unknown 0xFD, Pc JUMPDEST,
-  Stack (PUSH_N [0, 0x66]), Stack (PUSH_N [0, 0x87]), Pc JUMP, Pc JUMPDEST, Misc STOP, Pc JUMPDEST,
-  Info CALLVALUE, Arith ISZERO, Stack (PUSH_N [0, 0x73]), Pc JUMPI, Stack (PUSH_N [0]), Dup 0, Unknown 0xFD,
-  Pc JUMPDEST, Stack (PUSH_N [0, 0x7B]), Stack (PUSH_N [1, 0x1E]), Pc JUMP, Pc JUMPDEST, Misc STOP,
-  Pc JUMPDEST, Stack (PUSH_N [0, 0x85]), Stack (PUSH_N [1, 0xB4]), Pc JUMP, Pc JUMPDEST, Misc STOP,
-  Pc JUMPDEST, Stack (PUSH_N [2]), Stack (PUSH_N [0]), Swap 0, Storage SLOAD, Swap 0, Stack (PUSH_N [1, 0]),
-  Arith EXP, Swap 0, Arith DIV,
+  Stack (PUSH_N [0]), Stack CALLDATALOAD, Arith DIV, Bits inst_AND, Stack (PUSH_N [0x1B, 0x92, 0x65, 0xB8]),
+  Dup 1, Arith inst_EQ, Stack (PUSH_N [0, 0x5B]), Pc JUMPI, Dup 0, Stack (PUSH_N [0x59, 0xE, 0x1A, 0xE3]),
+  Arith inst_EQ, Stack (PUSH_N [0, 0x70]), Pc JUMPI, Dup 0, Stack (PUSH_N [0x8F, 0x95, 0x95, 0xD4]),
+  Arith inst_EQ, Stack (PUSH_N [0, 0x83]), Pc JUMPI, Pc JUMPDEST, Stack (PUSH_N [0]), Dup 0, Unknown 0xFD,
+  Pc JUMPDEST, Info CALLVALUE, Arith ISZERO, Stack (PUSH_N [0, 0x66]), Pc JUMPI, Stack (PUSH_N [0]), Dup 0,
+  Unknown 0xFD, Pc JUMPDEST, Stack (PUSH_N [0, 0x6E]), Stack (PUSH_N [0, 0x8B]), Pc JUMP, Pc JUMPDEST,
+  Misc STOP, Pc JUMPDEST, Info CALLVALUE, Arith ISZERO, Stack (PUSH_N [0, 0x7B]), Pc JUMPI,
+  Stack (PUSH_N [0]), Dup 0, Unknown 0xFD, Pc JUMPDEST, Stack (PUSH_N [0, 0x6E]), Stack (PUSH_N [0, 0xCE]),
+  Pc JUMP, Pc JUMPDEST, Stack (PUSH_N [0, 0x6E]), Stack (PUSH_N [1, 0x11]), Pc JUMP, Pc JUMPDEST,
+  Stack (PUSH_N [2]), Storage SLOAD, Info CALLER,
   Stack (PUSH_N
           [0xFF, 0xFF, 0xFF, 0xFF, 0xFF, 0xFF, 0xFF, 0xFF, 0xFF, 0xFF, 0xFF, 0xFF, 0xFF, 0xFF, 0xFF, 0xFF,
            0xFF, 0xFF, 0xFF, 0xFF]),
-  Bits inst_AND,
+  Swap 0, Dup 1, Bits inst_AND, Swap 1, Bits inst_AND, Arith inst_EQ, Stack (PUSH_N [0, 0xB3]), Pc JUMPI,
+  Stack (PUSH_N [0]), Dup 0, Unknown 0xFD, Pc JUMPDEST, Stack (PUSH_N [1]), Storage SLOAD,
   Stack (PUSH_N
           [0xFF, 0xFF, 0xFF, 0xFF, 0xFF, 0xFF, 0xFF, 0xFF, 0xFF, 0xFF, 0xFF, 0xFF, 0xFF, 0xFF, 0xFF, 0xFF,
            0xFF, 0xFF, 0xFF, 0xFF]),
-  Bits inst_AND, Info CALLER,
+  Bits inst_AND, Misc SUICIDE, Pc JUMPDEST, Stack (PUSH_N [2]), Storage SLOAD, Info CALLER,
   Stack (PUSH_N
           [0xFF, 0xFF, 0xFF, 0xFF, 0xFF, 0xFF, 0xFF, 0xFF, 0xFF, 0xFF, 0xFF, 0xFF, 0xFF, 0xFF, 0xFF, 0xFF,
            0xFF, 0xFF, 0xFF, 0xFF]),
-  Bits inst_AND, Arith inst_EQ, Arith ISZERO, Arith ISZERO, Stack (PUSH_N [0, 0xE3]), Pc JUMPI,
-  Stack (PUSH_N [0]), Dup 0, Unknown 0xFD, Pc JUMPDEST, Stack (PUSH_N [1]), Stack (PUSH_N [0]), Swap 0,
-  Storage SLOAD, Swap 0, Stack (PUSH_N [1, 0]), Arith EXP, Swap 0, Arith DIV,
+  Swap 0, Dup 1, Bits inst_AND, Swap 1, Bits inst_AND, Arith inst_EQ, Stack (PUSH_N [0, 0xF6]), Pc JUMPI,
+  Stack (PUSH_N [0]), Dup 0, Unknown 0xFD, Pc JUMPDEST, Stack (PUSH_N [0]), Storage SLOAD,
   Stack (PUSH_N
           [0xFF, 0xFF, 0xFF, 0xFF, 0xFF, 0xFF, 0xFF, 0xFF, 0xFF, 0xFF, 0xFF, 0xFF, 0xFF, 0xFF, 0xFF, 0xFF,
            0xFF, 0xFF, 0xFF, 0xFF]),
-  Bits inst_AND,
+  Bits inst_AND, Misc SUICIDE, Pc JUMPDEST, Stack (PUSH_N [0]), Storage SLOAD, Info CALLER,
   Stack (PUSH_N
           [0xFF, 0xFF, 0xFF, 0xFF, 0xFF, 0xFF, 0xFF, 0xFF, 0xFF, 0xFF, 0xFF, 0xFF, 0xFF, 0xFF, 0xFF, 0xFF,
            0xFF, 0xFF, 0xFF, 0xFF]),
-  Bits inst_AND, Misc SUICIDE, Pc JUMPDEST, Stack (PUSH_N [2]), Stack (PUSH_N [0]), Swap 0, Storage SLOAD,
-  Swap 0, Stack (PUSH_N [1, 0]), Arith EXP, Swap 0, Arith DIV,
-  Stack (PUSH_N
-          [0xFF, 0xFF, 0xFF, 0xFF, 0xFF, 0xFF, 0xFF, 0xFF, 0xFF, 0xFF, 0xFF, 0xFF, 0xFF, 0xFF, 0xFF, 0xFF,
-           0xFF, 0xFF, 0xFF, 0xFF]),
-  Bits inst_AND,
-  Stack (PUSH_N
-          [0xFF, 0xFF, 0xFF, 0xFF, 0xFF, 0xFF, 0xFF, 0xFF, 0xFF, 0xFF, 0xFF, 0xFF, 0xFF, 0xFF, 0xFF, 0xFF,
-           0xFF, 0xFF, 0xFF, 0xFF]),
-  Bits inst_AND, Info CALLER,
-  Stack (PUSH_N
-          [0xFF, 0xFF, 0xFF, 0xFF, 0xFF, 0xFF, 0xFF, 0xFF, 0xFF, 0xFF, 0xFF, 0xFF, 0xFF, 0xFF, 0xFF, 0xFF,
-           0xFF, 0xFF, 0xFF, 0xFF]),
-  Bits inst_AND, Arith inst_EQ, Arith ISZERO, Arith ISZERO, Stack (PUSH_N [1, 0x7A]), Pc JUMPI,
-  Stack (PUSH_N [0]), Dup 0, Unknown 0xFD, Pc JUMPDEST, Stack (PUSH_N [0]), Dup 0, Swap 0, Storage SLOAD,
-  Swap 0, Stack (PUSH_N [1, 0]), Arith EXP, Swap 0, Arith DIV,
-  Stack (PUSH_N
-          [0xFF, 0xFF, 0xFF, 0xFF, 0xFF, 0xFF, 0xFF, 0xFF, 0xFF, 0xFF, 0xFF, 0xFF, 0xFF, 0xFF, 0xFF, 0xFF,
-           0xFF, 0xFF, 0xFF, 0xFF]),
-  Bits inst_AND,
-  Stack (PUSH_N
-          [0xFF, 0xFF, 0xFF, 0xFF, 0xFF, 0xFF, 0xFF, 0xFF, 0xFF, 0xFF, 0xFF, 0xFF, 0xFF, 0xFF, 0xFF, 0xFF,
-           0xFF, 0xFF, 0xFF, 0xFF]),
-  Bits inst_AND, Misc SUICIDE, Pc JUMPDEST, Stack (PUSH_N [0]), Dup 0, Swap 0, Storage SLOAD, Swap 0,
-  Stack (PUSH_N [1, 0]), Arith EXP, Swap 0, Arith DIV,
-  Stack (PUSH_N
-          [0xFF, 0xFF, 0xFF, 0xFF, 0xFF, 0xFF, 0xFF, 0xFF, 0xFF, 0xFF, 0xFF, 0xFF, 0xFF, 0xFF, 0xFF, 0xFF,
-           0xFF, 0xFF, 0xFF, 0xFF]),
-  Bits inst_AND,
-  Stack (PUSH_N
-          [0xFF, 0xFF, 0xFF, 0xFF, 0xFF, 0xFF, 0xFF, 0xFF, 0xFF, 0xFF, 0xFF, 0xFF, 0xFF, 0xFF, 0xFF, 0xFF,
-           0xFF, 0xFF, 0xFF, 0xFF]),
-  Bits inst_AND, Info CALLER,
-  Stack (PUSH_N
-          [0xFF, 0xFF, 0xFF, 0xFF, 0xFF, 0xFF, 0xFF, 0xFF, 0xFF, 0xFF, 0xFF, 0xFF, 0xFF, 0xFF, 0xFF, 0xFF,
-           0xFF, 0xFF, 0xFF, 0xFF]),
-  Bits inst_AND, Arith inst_EQ, Arith ISZERO, Arith ISZERO, Stack (PUSH_N [2, 0xF]), Pc JUMPI,
+  Swap 0, Dup 1, Bits inst_AND, Swap 1, Bits inst_AND, Arith inst_EQ, Stack (PUSH_N [1, 0x39]), Pc JUMPI,
   Stack (PUSH_N [0]), Dup 0, Unknown 0xFD, Pc JUMPDEST, Pc JUMP, Misc STOP, Log LOG1,
-  Stack (PUSH_N [0x62, 0x7A, 0x7A, 0x72, 0x30, 0x58]), Arith SHA3, Unknown 0xCD,
+  Stack (PUSH_N [0x62, 0x7A, 0x7A, 0x72, 0x30, 0x58]), Arith SHA3,
   Stack (PUSH_N
-          [0x38, 0xDB, 0x5B, 0xAD, 0xA1, 0x13, 0xDE, 0x91, 0xEC, 0x97, 0x9B, 0x4D, 0xCA, 0x8F, 0xDC, 0xB3,
-           0xC6, 0x16, 0xA0, 5, 0x62, 0xA6, 0x7F, 0x5C, 0x28, 0x8A]),
-  Stack (PUSH_N [0xC4, 0x79, 0xD1, 0, 0x29])]"
-(* 159 instructions *)
+          [0xD2, 0xEE, 0x80, 0x51, 0xB0, 0x98, 0xC7, 0x99, 0xDF, 0x41, 0x46, 0x65, 0x99, 0xCD, 0x31, 0x1E,
+           0x37, 0x6F, 0xD3, 0x63, 0x72, 0xF2, 0xBE, 0xCE, 0xC0, 0x8F, 0xE4, 0x94]),
+  Unknown 0xBA, Memory EXTCODECOPY, Unknown 0xC1, Misc STOP, Unknown 0x29]"
+(* 135 instructions *)
 
 lemma
- "parse_bytecode ''60606040526000357c0100000000000000000000000000000000000000000000000000000000900463ffffffff1680631b9265b814610053578063590e1ae3146100685780638f9595d41461007d57600080fd5b341561005e57600080fd5b610066610087565b005b341561007357600080fd5b61007b61011e565b005b6100856101b4565b005b600260009054906101000a900473ffffffffffffffffffffffffffffffffffffffff1673ffffffffffffffffffffffffffffffffffffffff163373ffffffffffffffffffffffffffffffffffffffff161415156100e357600080fd5b600160009054906101000a900473ffffffffffffffffffffffffffffffffffffffff1673ffffffffffffffffffffffffffffffffffffffff16ff5b600260009054906101000a900473ffffffffffffffffffffffffffffffffffffffff1673ffffffffffffffffffffffffffffffffffffffff163373ffffffffffffffffffffffffffffffffffffffff1614151561017a57600080fd5b6000809054906101000a900473ffffffffffffffffffffffffffffffffffffffff1673ffffffffffffffffffffffffffffffffffffffff16ff5b6000809054906101000a900473ffffffffffffffffffffffffffffffffffffffff1673ffffffffffffffffffffffffffffffffffffffff163373ffffffffffffffffffffffffffffffffffffffff1614151561020f57600080fd5b5600a165627a7a72305820cd7938db5bada113de91ec979b4dca8fdcb3c616a00562a67f5c288a71c479d10029'' = insts_ex"
+ "parse_bytecode ''6060604052600436106100565763ffffffff7c01000000000000000000000000000000000000000000000000000000006000350416631b9265b8811461005b578063590e1ae3146100705780638f9595d414610083575b600080fd5b341561006657600080fd5b61006e61008b565b005b341561007b57600080fd5b61006e6100ce565b61006e610111565b6002543373ffffffffffffffffffffffffffffffffffffffff9081169116146100b357600080fd5b60015473ffffffffffffffffffffffffffffffffffffffff16ff5b6002543373ffffffffffffffffffffffffffffffffffffffff9081169116146100f657600080fd5b60005473ffffffffffffffffffffffffffffffffffffffff16ff5b6000543373ffffffffffffffffffffffffffffffffffffffff90811691161461013957600080fd5b5600a165627a7a723058207bd2ee8051b098c799df41466599cd311e376fd36372f2becec08fe494ba3cc10029'' = insts_ex"
   unfolding insts_ex_def
   by eval
 
 definition "blocks_escrow == build_blocks insts_ex"
+
+lemma blocks_escrow_simp:
+ "blocks_escrow = [(0, [(0, Stack (PUSH_N [0x60])), (2, Stack (PUSH_N [0x40])), (4, Memory MSTORE), (5, Stack (PUSH_N [4])),
+       (7, Info CALLDATASIZE), (8, Arith inst_LT), (9, Stack (PUSH_N [0, 0x56]))],
+   Jumpi),
+  (13, [(13, Stack (PUSH_N [0xFF, 0xFF, 0xFF, 0xFF])),
+        (18, Stack (PUSH_N
+                     [1, 0, 0, 0, 0, 0, 0, 0, 0, 0, 0, 0, 0, 0, 0, 0, 0, 0, 0, 0, 0, 0, 0, 0, 0, 0, 0, 0,
+                      0])),
+        (48, Stack (PUSH_N [0])), (50, Stack CALLDATALOAD), (51, Arith DIV), (52, Bits inst_AND),
+        (53, Stack (PUSH_N [0x1B, 0x92, 0x65, 0xB8])), (58, Dup 1), (59, Arith inst_EQ),
+        (60, Stack (PUSH_N [0, 0x5B]))],
+   Jumpi),
+  (64, [(64, Dup 0), (65, Stack (PUSH_N [0x59, 0xE, 0x1A, 0xE3])), (70, Arith inst_EQ),
+        (71, Stack (PUSH_N [0, 0x70]))],
+   Jumpi),
+  (75, [(75, Dup 0), (76, Stack (PUSH_N [0x8F, 0x95, 0x95, 0xD4])), (81, Arith inst_EQ),
+        (82, Stack (PUSH_N [0, 0x83]))],
+   Jumpi),
+  (86, [(86, Pc JUMPDEST), (87, Stack (PUSH_N [0])), (89, Dup 0), (90, Unknown 0xFD)], Terminal),
+  (91, [(91, Pc JUMPDEST), (92, Info CALLVALUE), (93, Arith ISZERO), (94, Stack (PUSH_N [0, 0x66]))], Jumpi),
+  (98, [(98, Stack (PUSH_N [0])), (100, Dup 0), (101, Unknown 0xFD)], Terminal),
+  (102, [(102, Pc JUMPDEST), (103, Stack (PUSH_N [0, 0x6E])), (106, Stack (PUSH_N [0, 0x8B]))], Jump),
+  (110, [(110, Pc JUMPDEST), (111, Misc STOP)], Terminal),
+  (112, [(112, Pc JUMPDEST), (113, Info CALLVALUE), (114, Arith ISZERO), (115, Stack (PUSH_N [0, 0x7B]))],
+   Jumpi),
+  (119, [(119, Stack (PUSH_N [0])), (121, Dup 0), (122, Unknown 0xFD)], Terminal),
+  (123, [(123, Pc JUMPDEST), (124, Stack (PUSH_N [0, 0x6E])), (127, Stack (PUSH_N [0, 0xCE]))], Jump),
+  (131, [(131, Pc JUMPDEST), (132, Stack (PUSH_N [0, 0x6E])), (135, Stack (PUSH_N [1, 0x11]))], Jump),
+  (139, [(139, Pc JUMPDEST), (140, Stack (PUSH_N [2])), (142, Storage SLOAD), (143, Info CALLER),
+         (144, Stack (PUSH_N
+                       [0xFF, 0xFF, 0xFF, 0xFF, 0xFF, 0xFF, 0xFF, 0xFF, 0xFF, 0xFF, 0xFF, 0xFF, 0xFF, 0xFF,
+                        0xFF, 0xFF, 0xFF, 0xFF, 0xFF, 0xFF])),
+         (165, Swap 0), (166, Dup 1), (167, Bits inst_AND), (168, Swap 1), (169, Bits inst_AND),
+         (170, Arith inst_EQ), (171, Stack (PUSH_N [0, 0xB3]))],
+   Jumpi),
+  (175, [(175, Stack (PUSH_N [0])), (177, Dup 0), (178, Unknown 0xFD)], Terminal),
+  (179, [(179, Pc JUMPDEST), (180, Stack (PUSH_N [1])), (182, Storage SLOAD),
+         (183, Stack (PUSH_N
+                       [0xFF, 0xFF, 0xFF, 0xFF, 0xFF, 0xFF, 0xFF, 0xFF, 0xFF, 0xFF, 0xFF, 0xFF, 0xFF, 0xFF,
+                        0xFF, 0xFF, 0xFF, 0xFF, 0xFF, 0xFF])),
+         (204, Bits inst_AND), (205, Misc SUICIDE)],
+   Terminal),
+  (206, [(206, Pc JUMPDEST), (207, Stack (PUSH_N [2])), (209, Storage SLOAD), (210, Info CALLER),
+         (211, Stack (PUSH_N
+                       [0xFF, 0xFF, 0xFF, 0xFF, 0xFF, 0xFF, 0xFF, 0xFF, 0xFF, 0xFF, 0xFF, 0xFF, 0xFF, 0xFF,
+                        0xFF, 0xFF, 0xFF, 0xFF, 0xFF, 0xFF])),
+         (232, Swap 0), (233, Dup 1), (234, Bits inst_AND), (235, Swap 1), (236, Bits inst_AND),
+         (237, Arith inst_EQ), (238, Stack (PUSH_N [0, 0xF6]))],
+   Jumpi),
+  (242, [(242, Stack (PUSH_N [0])), (244, Dup 0), (245, Unknown 0xFD)], Terminal),
+  (246, [(246, Pc JUMPDEST), (247, Stack (PUSH_N [0])), (249, Storage SLOAD),
+         (250, Stack (PUSH_N
+                       [0xFF, 0xFF, 0xFF, 0xFF, 0xFF, 0xFF, 0xFF, 0xFF, 0xFF, 0xFF, 0xFF, 0xFF, 0xFF, 0xFF,
+                        0xFF, 0xFF, 0xFF, 0xFF, 0xFF, 0xFF])),
+         (271, Bits inst_AND), (272, Misc SUICIDE)],
+   Terminal),
+  (273, [(273, Pc JUMPDEST), (274, Stack (PUSH_N [0])), (276, Storage SLOAD), (277, Info CALLER),
+         (278, Stack (PUSH_N
+                       [0xFF, 0xFF, 0xFF, 0xFF, 0xFF, 0xFF, 0xFF, 0xFF, 0xFF, 0xFF, 0xFF, 0xFF, 0xFF, 0xFF,
+                        0xFF, 0xFF, 0xFF, 0xFF, 0xFF, 0xFF])),
+         (299, Swap 0), (300, Dup 1), (301, Bits inst_AND), (302, Swap 1), (303, Bits inst_AND),
+         (304, Arith inst_EQ), (305, Stack (PUSH_N [1, 0x39]))],
+   Jumpi),
+  (309, [(309, Stack (PUSH_N [0])), (311, Dup 0), (312, Unknown 0xFD)], Terminal),
+  (313, [(313, Pc JUMPDEST)], Jump), (315, [(315, Misc STOP)], Terminal),
+  (316, [(316, Log LOG1), (317, Stack (PUSH_N [0x62, 0x7A, 0x7A, 0x72, 0x30, 0x58])), (324, Arith SHA3),
+         (325, Stack (PUSH_N
+                       [0xD2, 0xEE, 0x80, 0x51, 0xB0, 0x98, 0xC7, 0x99, 0xDF, 0x41, 0x46, 0x65, 0x99, 0xCD,
+                        0x31, 0x1E, 0x37, 0x6F, 0xD3, 0x63, 0x72, 0xF2, 0xBE, 0xCE, 0xC0, 0x8F, 0xE4, 0x94])),
+         (354, Unknown 0xBA)],
+   Terminal),
+  (355, [(355, Memory EXTCODECOPY), (356, Unknown 0xC1)], Terminal), (357, [(357, Misc STOP)], Terminal),
+  (358, [(358, Unknown 0x29)], Terminal)]"
+  by eval
+
 definition addfund_hash :: "32 word"  where
  "addfund_hash = 0x8f9595d4"
 
@@ -142,9 +178,6 @@ definition pay_hash :: "32 word"  where
 definition refund_hash :: "32 word"  where
  "refund_hash = 0x590e1ae3"
 
-definition
- "contract_fail \<equiv> ContractFail [ShouldNotHappen]"
-
 definition return_action ::"address \<Rightarrow> address \<Rightarrow> address \<Rightarrow> address \<Rightarrow> 32 word \<Rightarrow> contract_action" where
   "return_action sender from to owner hash  = 
  (if hash = addfund_hash \<and> sender = from then
@@ -153,9 +186,25 @@ definition return_action ::"address \<Rightarrow> address \<Rightarrow> address 
     ContractSuicide from
   else if hash = pay_hash \<and> sender = owner then
     ContractSuicide to
-  else contract_fail)"
+  else
+    ContractFail [ShouldNotHappen])"
 
-lemma verify_escrow_return:
+context
+notes
+  words_simps[simp add]
+  calldataload_simps[simp add]
+  M_def[simp add]
+  Cmem_def[simp add]
+  memory_range.simps[simp del]
+ if_split[ split del ] sep_fun_simps[simp del]
+gas_value_simps[simp add] pure_emp_simps[simp add]
+evm_fun_simps[simp add] sep_lc[simp del] sep_conj_first[simp add]
+pure_false_simps[simp add] iszero_stack_def[simp add]
+begin
+
+theorem verify_escrow_return:
+notes
+  bit_mask_rev[simp add]
 shows
 "\<exists>r. triple 
   (program_counter 0 ** stack_height 0 ** (sent_data (word_rsplit (hash::32 word)::byte list))
@@ -167,7 +216,12 @@ shows
    ** memory (word_rcat [64::byte]) (word_rcat [x::byte]::256 word) **
    memory (word_rcat [96::byte]) (word_rcat [y::byte]::256 word))
   blocks_escrow (action (return_action sender from to owner hash) ** r)"
+  apply (simp add:blocks_escrow_simp)
   apply(simp add: return_action_def blocks_simps triple_def addfund_hash_def refund_hash_def pay_hash_def)
+apply(split if_split, rule conjI)
+   apply(rule impI, ((erule conjE)+)?, rule exI)
+ apply((block_vcg)+)[1]
+ apply(sep_cancel)+
 
   oops
 
